Update verification examples

nola/examples/later.v
@@ -7,13 +7,6 @@ Import WpwNotation.
 
 Implicit Type (N : namespace) (l : loc).
 
-(** ** Linked list mutation *)
-
-(** Target function *)
-Definition iter_ilist : val := rec: "self" "f" "c" "l" :=
-  if: !"c" ≤ #0 then #() else
-    "f" "l";; "c" <- !"c" - #1;; "self" "f" "c" (!("l" +ₗ #1)).
-
 Section verify.
   Context `{!inv'GS (▶ ∙) Σ, !heapGS_gen hlc Σ}.
 
@@ -34,7 +27,27 @@ Section verify.
   Instance ilist_persistent N Φ l : Persistent (ilist N Φ l).
   Proof. rewrite ilist_unfold. exact _. Qed.
 
-  (** Safety of [iter] *)
+  (** Access the tail of [ilist] *)
+  Definition tail_ilist : val := λ: "l", let: "l'" := !("l" +ₗ #1) in "l'".
+  Lemma wp_tail_ilist {N Φ l} :
+    {{{ ilist N Φ l }}}[inv_wsat laterl]
+      tail_ilist #l @ ↑N
+    {{{ l', RET #l'; ilist N Φ l' }}}.
+  Proof.
+    iIntros (Ψ) "#l →Ψ". wp_rec. wp_pure. wp_bind (! _)%E.
+    rewrite ilist_unfold. iDestruct "l" as "[ihd itl]".
+    iMod (inv_tok_acc (FML:=▶ ∙) (sm:=laterl) with "itl") as
+      "/=[(%l' & >↦l' & #ltl) cl]"; [done|].
+    wp_load. iModIntro. iMod ("cl" with "[↦l']") as "_".
+    { iExists _. by iFrame. }
+    iModIntro. wp_pures. iApply ("→Ψ" with "ltl").
+  Qed.
+
+  (** Iterate over [ilist] *)
+  Definition iter_ilist : val := rec: "self" "f" "c" "l" :=
+    if: !"c" ≤ #0 then #() else
+      "f" "l";; "c" <- !"c" - #1;;
+      let: "l'" := tail_ilist "l" in "self" "f" "c" "l'".
   Lemma wp_iter_list {N Φ c l} {f : val} {n : nat} :
     (∀ l0, {{{ inv_tok N (Next (Φ l0)) }}}[inv_wsat laterl] f #l0 @ ↑N
       {{{ RET #(); True }}}) -∗
@@ -42,15 +55,13 @@ Section verify.
       iter_ilist f #c #l @ ↑N
     {{{ RET #(); c ↦ #0 }}}.
   Proof.
-    iIntros "#f" (Ψ) "!> [c↦ #l] →Ψ". iInduction n as [|m] "IH" forall (l) "l".
+    iIntros "#f" (Ψ) "!> /=[c↦ #l] →Ψ".
+    iInduction n as [|m] "IH" forall (l) "l".
     { wp_rec. wp_load. wp_pures. by iApply "→Ψ". }
-    rewrite ilist_unfold. iDestruct "l" as "[ihd itl]". wp_rec. wp_load.
-    wp_pures. wp_apply "f"; [done|]. iIntros "_". wp_load. wp_store. wp_op.
-    wp_bind (! _)%E. have -> : (S m - 1)%Z = m by lia.
-    iMod (inv_tok_acc (FML:=▶ ∙) (sm:=laterl) with "itl") as
-      "/=[(%l' & ↦l' & #l') cl]"; [done|].
-    wp_load. iModIntro. iMod ("cl" with "[↦l']") as "_".
-    { iNext. iExists _. by iFrame "↦l'". }
-    iModIntro. by iApply ("IH" with "c↦ →Ψ").
+    wp_rec. wp_load. wp_pures. wp_apply "f".
+    { rewrite ilist_unfold. iDestruct "l" as "[$ _]". }
+    iIntros "_". wp_load. wp_store. have -> : (S m - 1)%Z = m by lia.
+    wp_apply wp_tail_ilist; [done|]. iIntros (l') "#ltl". wp_pures.
+    iApply ("IH" with "c↦ →Ψ ltl").
   Qed.
 End verify.
